Add test for Class.Functional.Relation

rocq/ZF/Meta/Decl/Class/Relation/Functional.v
@@ -1,6 +1,7 @@
 Require Import Coq.Lists.List.
 Require Import Coq.Strings.String.
 
+Require Import ZF.Meta.DeclP.
 Require Import ZF.Meta.DeclT.
 Require Import ZF.Meta.Env.
 Require Import ZF.Meta.Syntax.
@@ -9,17 +10,87 @@ Require Import ZF.Meta.Ty.
 Import ListNotations.
 Open Scope string_scope.
 
-(* Functional F : Prop.                                                         *)
+Require Import ZF.Meta.Decl.Class.Equiv.
+Require Import ZF.Meta.Decl.Class.Incl.
+Require Import ZF.Meta.Decl.Class.Relation.FunctionalAt.
+Require Import ZF.Meta.Decl.Set.OrdPair.
+
+(* Functional F <-> forall x y z, F :(x,y): -> F :(x,z): -> y = z.              *)
 Definition Functional : DeclT :=
   {| paraT := [TyClass]
   ;  resT  := TyProp
-  ;  bodyT := HoleT TyProp
+  ;  bodyT :=
+      All
+        (All
+          (All
+            (Imp
+              (App (Var 3)
+                (IdentT (Name.local "ordPair") (args [Var 2; Var 1])))
+              (Imp
+                (App (Var 3)
+                  (IdentT (Name.local "ordPair") (args [Var 2; Var 0])))
+                (Syntax.Equal (Var 1) (Var 0))))))
   |}.
 
-Definition imports : Env := Env.empty.
+(* forall F G, equiv F G -> Functional F -> Functional G.                       *)
+Definition EquivCompat : DeclP :=
+  let concl :=
+    Imp
+      (IdentT (Name.local "equiv") (args [Var 1; Var 0]))
+      (Imp
+        (IdentT (Name.local "Functional") (args [Var 1]))
+        (IdentT (Name.local "Functional") (args [Var 0])))
+  in
+    {| paraP  := [TyClass; TyClass]
+    ;  conclP := concl
+    ;  bodyP  := HoleP concl
+    |}.
 
-Definition exports : Env := Env.fromListT
-  [ (Name.local "Functional", Functional)
+(* forall F G, Incl F G -> Functional G -> Functional F.                        *)
+Definition InclCompat : DeclP :=
+  let concl :=
+    Imp
+      (IdentT (Name.local "Incl") (args [Var 1; Var 0]))
+      (Imp
+        (IdentT (Name.local "Functional") (args [Var 0]))
+        (IdentT (Name.local "Functional") (args [Var 1])))
+  in
+    {| paraP  := [TyClass; TyClass]
+    ;  conclP := concl
+    ;  bodyP  := HoleP concl
+    |}.
+
+(* forall F, Functional F <-> forall a, FunctionalAt F a.                       *)
+Definition IsFunctionalAt : DeclP :=
+  let concl :=
+    Iff
+      (IdentT (Name.local "Functional") (args [Var 0]))
+      (All
+        (IdentT (Name.local "FunctionalAt") (args [Var 1; Var 0])))
+  in
+    {| paraP  := [TyClass]
+    ;  conclP := concl
+    ;  bodyP  := HoleP concl
+    |}.
+
+(* Environment.                                                                 *)
+
+Definition imports : Env := Env.unions
+  [ Env.unqualify Equiv.exports
+  ; Env.unqualify Incl.exports
+  ; Env.unqualify FunctionalAt.exports
+  ; Env.unqualify OrdPair.exports
+  ].
+
+Definition exports : Env := Env.unions
+  [ Env.fromListT
+      [ (Name.local "Functional", Functional)
+      ]
+  ; Env.fromListP
+      [ (Name.local "EquivCompat"   , EquivCompat)
+      ; (Name.local "InclCompat"    , InclCompat)
+      ; (Name.local "IsFunctionalAt", IsFunctionalAt)
+      ]
   ].
 
 Definition env : Env := Env.union imports exports.
